symbolic/symbolic.v
@@ -1,7 +1,7 @@
 Require Import Ssreflect.ssreflect Ssreflect.ssrfun Ssreflect.ssrbool Ssreflect.eqtype Ssreflect.ssrnat Ssreflect.seq.
 Require Import CoqUtils.hseq CoqUtils.word CoqUtils.partmap.
 
-Require Import lib.utils common.types.
+Require Import lib.utils lib.hseq_utils common.types.
 
 Set Implicit Arguments.
 Unset Strict Implicit.
@@ -105,43 +105,29 @@ Definition tag_type tk :=
   | M => mem_tag_type tty
   end.
 
+Definition type_of_result (o : option tag_kind) :=
+  odflt [eqType of unit] (option_map tag_type o).
+
 Definition instr_tag (op : vopcode) :=
   match op with
   | SERVICE => entry_tag_type tty
   | _ => mem_tag_type tty
   end.
 
-Record ivec : Type := IVec {
-  op  : vopcode;
+Record mvec (op : vopcode) : Type := MVec {
   tpc : tag_type P;
   ti  : instr_tag op;
   ts  : hseq tag_type (vinputs op)
 }.
 
-Lemma ivec_eq_inv op op' tpc tpc' ti ti' ts ts'
-                  (p : @IVec op tpc ti ts = @IVec op' tpc' ti' ts') :
-  [/\ op = op', tpc = tpc',
-      Tagged instr_tag ti = Tagged instr_tag ti' &
-      Tagged (hseq tag_type \o vinputs) ts = existT _ op' ts'].
-Proof. inversion p. by constructor. Qed.
-
-Definition type_of_result (o : option tag_kind) :=
-  odflt [eqType of unit] (option_map tag_type o).
-
-Record ovec (op : opcode) : Type := OVec {
-  trpc : tag_type P;
-  tr   : type_of_result (outputs op)
-}.
-
-Definition vovec (vop : vopcode) : Type :=
-  match vop with
-  | OP op => ovec op
-  | SERVICE => unit
-  end.
+Lemma mvec_eq_inv op tpc tpc' ti ti' ts ts'
+                  (p : @MVec op tpc ti ts = @MVec op tpc' ti' ts') :
+  [/\ tpc = tpc', ti = ti' & ts = ts'].
+Proof. by case: p. Qed.
 
 End WithTagTypes.
 
-Arguments IVec {_} _ _ _ _.
+Arguments MVec {_} _ _ _ _.
 
 Open Scope bool_scope.
 
@@ -153,7 +139,7 @@ Context (mt : machine_types)
 Class params := {
   ttypes :> tag_types;
 
-  transfer : forall (iv : ivec ttypes), option (vovec ttypes (op iv));
+  transfer : forall op : vopcode, mvec ttypes op -> option (mvec ttypes op);
 
   internal_state : eqType
 }.
@@ -195,121 +181,150 @@ Definition syscall_table := {partmap mword mt -> syscall}.
 Variable table : syscall_table.
 
 Definition run_syscall (sc : syscall) (st : state) : option state :=
-  match transfer (IVec SERVICE (taga (pc st)) (entry_tag sc) [hseq]) with
+  match transfer (MVec SERVICE (taga (pc st)) (entry_tag sc) [hseq]) with
   | Some _ => sem sc st
   | None => None
   end.
 
-Definition next_state (st : state) (iv : ivec ttypes)
-                      (k : vovec ttypes (op iv) -> option state) : option state :=
-  do! ov <- transfer iv;
-    k ov.
+Definition tag_loc tk :=
+  match tk with
+  | P => unit
+  | R => reg mt
+  | M => mword mt
+  end.
 
-Definition next_state_reg_and_pc (st : state) (iv : @ivec ttypes)
-  (r : reg mt) (x : word) (pc' : word) : option state :=
-  next_state st (
-    match op iv as o return vovec _ o -> option state with
-    | OP op => fun ov =>
-      match outputs op as o return (type_of_result _ o -> option state) with
-        | Some R => fun tr' =>
-            do! regs' <- updm (regs st) r x@tr';
-            Some (State (mem st) regs' pc'@(trpc ov) (internal st))
-        | _ => fun _ => None
-      end (tr ov)
-    | SERVICE => fun _ => None
-    end
-  ).
+Definition tag_get (tk : tag_kind) : tag_loc tk -> state -> option (tag_type ttypes tk) :=
+  match tk with
+    | P => fun _ s => Some (pct s)
+    | R => fun r s => omap taga (getm (regs s) r)
+    | M => fun p s => omap taga (getm (mem  s) p)
+  end.
 
-Definition next_state_reg (st : state) (mvec : @ivec ttypes) r x : option state :=
-  next_state_reg_and_pc st mvec r x (vala (pc st)).+1.
+Definition tag_get_from (s : state) : forall tk, tag_loc tk -> option (tag_type ttypes tk) :=
+  fun _ l => tag_get l s.
 
-Definition next_state_pc (st : state) (iv : @ivec ttypes)
-  (x : word) : option state :=
-  next_state st (
-    match op iv as o return vovec _ o -> option state with
-    | OP op => fun ov =>
-                 Some (State (mem st) (regs st) x@(trpc ov) (internal st))
-    | SERVICE => fun _ => None
-    end
-  ).
+Definition tag_upd (tk : tag_kind) : tag_loc tk -> tag_type ttypes tk -> state -> option state :=
+  match tk with
+    | P => fun _ t s => Some (State (mem s) (regs s) (pcv s)@t (internal s))
+    | R => fun r t s => do! regs' <- repm (regs s) r (fun rvt => vala rvt @ t);
+                            Some (State (mem s) regs' (pc s) (internal s))
+    | M => fun p t s => do! mem' <- repm (mem s) p (fun rvt => vala rvt @ t);
+                            Some (State mem' (regs s) (pc s) (internal s))
+  end.
+
+(* Without the `Unset/Set Implicit Arguments` jiggery-pokery, `opL` and `lv`
+   become implicit and I can't figure out how to undo that.  Similarly,
+   functions that use an `mvec ttypes (opL lv)` argument treat the `lv` as
+   implicit. *)
+Unset Implicit Arguments.
+Record lvec : Type := LVec {
+  opL  : vopcode;
+  tpcL : tag_type ttypes P;
+  tiL  : instr_tag ttypes opL;
+  tsL  : hseq tag_loc (vinputs opL)
+}.
+
+Definition get_lvec (st : state) (lv : lvec) : option (mvec ttypes (opL lv)) :=
+  omap (MVec (opL lv) (tpcL lv) (tiL lv)) (hmapo (tag_get_from st) (tsL lv)).
+
+Definition set_lvec (st : state) (lv : lvec) (mv : mvec ttypes (opL lv)) : option state :=
+  let writeback_pc    := @tag_upd P tt (tpc mv) in
+  let writeback_instr := match opL lv as opL return instr_tag ttypes opL -> _ with
+                           | OP _    => @tag_upd M (pcv st)
+                           | SERVICE => fun _ _ => None (* Or Some? *)
+                         end (ti mv) in
+  let writebacks_args := hhomogeneous (hzipwith (@tag_upd) (tsL lv) (ts mv))
+  in foldr (@obind _ _) (Some st) [:: writeback_pc, writeback_instr & writebacks_args].
+
+Definition next_state (st : state) (lv : lvec) : option state :=
+  do! ivts <- hmapo (tag_get_from st) (tsL lv);
+  do! ov   <- transfer (MVec (opL lv) (tpcL lv) (tiL lv) ivts);
+  set_lvec st lv ov.
+Set Implicit Arguments.
+
+Definition next_state_pc (st : state) (lv : lvec) (pc' : word) : option state :=
+  do! st' <- next_state st lv;
+  Some (State (mem st') (regs st') pc'@(pct st') (internal st')).
+
+Definition next_state_reg_and_pc (st : state) (lv : lvec)
+                                 (r : reg mt) (x : word) (pc' : word) : option state :=
+  do! st'   <- next_state_pc st lv pc';
+  do! regs' <- repm (regs st') r (fun v => x@(taga v));
+  Some (State (mem st') regs' pc'@(pct st') (internal st')).
+
+Definition next_state_reg (st : state) (lv : lvec) (r : reg mt) (x : word) : option state :=
+  next_state_reg_and_pc st lv r x (vala (pc st)).+1.
 
 Inductive step (st st' : state) : Prop :=
 | step_nop : forall mem reg pc tpc i ti extra
     (ST   : st = State mem reg pc@tpc extra)
     (PC   : mem pc = Some i@ti)
     (INST : decode_instr i = Some (Nop _)),
-    let mvec := IVec NOP tpc ti [hseq] in forall
-    (NEXT : next_state_pc st mvec (pc.+1) = Some st'),    step st st'
-| step_const : forall mem reg pc tpc i ti n r old (told : tag_type ttypes R) extra
+    let lv := LVec NOP tpc ti [hseq] in forall
+    (NEXT : next_state_pc st lv (pc.+1) = Some st'),    step st st'
+| step_const : forall mem reg pc tpc i ti n r extra
     (ST   : st = State mem reg pc@tpc extra)
     (PC   : mem pc = Some i@ti)
-    (INST : decode_instr i = Some (Const n r))
-    (OLD  : reg r = Some old@told),
-    let mvec := IVec CONST tpc ti [hseq told] in forall
-    (NEXT : next_state_reg st mvec r (swcast n) = Some st'),   step st st'
-| step_mov : forall mem reg pc tpc i ti r1 w1 t1 r2 old told extra
+    (INST : decode_instr i = Some (Const n r)),
+    let lv := LVec CONST tpc ti [hseq r] in forall
+    (NEXT : next_state_reg st lv r (swcast n) = Some st'),   step st st'
+| step_mov : forall mem reg pc tpc i ti r1 r2 w1 extra
     (ST   : st = State mem reg pc@tpc extra)
     (PC   : mem pc = Some i@ti)
     (INST : decode_instr i = Some (Mov r1 r2))
-    (R1W  : reg r1 = Some w1@t1)
-    (OLD  : reg r2 = Some old@told),
-    let mvec := IVec MOV tpc ti [hseq t1; told] in forall
-    (NEXT : next_state_reg st mvec r2 w1 = Some st'),   step st st'
-| step_binop : forall mem reg pc tpc i ti op r1 r2 r3 w1 w2 t1 t2 old told extra
+    (R1W  : omap vala (reg r1) = Some w1),
+    let lv := LVec MOV tpc ti [hseq r1; r2] in forall
+    (NEXT : next_state_reg st lv r2 w1 = Some st'),   step st st'
+| step_binop : forall mem reg pc tpc i ti op r1 r2 r3 w1 w2 extra
     (ST   : st = State mem reg pc@tpc extra)
     (PC   : mem pc = Some i@ti)
     (INST : decode_instr i = Some (Binop op r1 r2 r3))
-    (R1W  : reg r1 = Some w1@t1)
-    (R2W  : reg r2 = Some w2@t2)
-    (OLD  : reg r3 = Some old@told),
-    let mvec := IVec (BINOP op) tpc ti [hseq t1; t2; told] in forall
-    (NEXT : next_state_reg st mvec r3 (binop_denote op w1 w2) = Some st'),
+    (R1W  : omap vala (reg r1) = Some w1)
+    (R2W  : omap vala (reg r2) = Some w2),
+    let lv := LVec (BINOP op) tpc ti [hseq r1; r2; r3] in forall
+    (NEXT : next_state_reg st lv r3 (binop_denote op w1 w2) = Some st'),
       step st st'
-| step_load : forall mem reg pc tpc i ti r1 r2 w1 w2 t1 t2 old told extra
+| step_load : forall mem reg pc tpc i ti r1 r2 w1 w2 extra
     (ST   : st = State mem reg pc@tpc extra)
     (PC   : mem pc = Some i@ti)
     (INST : decode_instr i = Some (Load r1 r2))
-    (R1W  : reg r1 = Some w1@t1)
-    (MEM1 : mem w1 = Some w2@t2)
-    (OLD  : reg r2 = Some old@told),
-    let mvec := IVec LOAD tpc ti [hseq t1; t2; told] in forall
-    (NEXT : next_state_reg st mvec r2 w2 = Some st'),    step st st'
-| step_store : forall mem reg pc i r1 r2 w1 w2 tpc ti t1 t2 old told extra
+    (R1W  : omap vala (reg r1) = Some w1)
+    (MEM1 : omap vala (mem w1) = Some w2),
+    let lv := LVec LOAD tpc ti [hseq r1; w1; r2] in forall
+    (NEXT : next_state_reg st lv r2 w2 = Some st'),    step st st'
+| step_store : forall mem reg pc tpc i ti r1 r2 w1 w2 extra
     (ST   : st = State mem reg pc@tpc extra)
     (PC   : mem pc = Some i@ti)
     (INST : decode_instr i = Some (Store r1 r2))
-    (R1W  : reg r1 = Some w1@t1)
-    (R2W  : reg r2 = Some w2@t2)
-    (OLD  : mem w1 = Some old@told),
-    let mvec := IVec STORE tpc ti [hseq t1; t2; told] in forall
-    (NEXT : @next_state st mvec (fun ov =>
-                 do! mem' <- updm mem w1 w2@(tr ov);
-                 Some (State mem' reg (pc.+1)@(trpc ov) extra)) = Some st'),
-              step st st'
-| step_jump : forall mem reg pc i r w tpc ti t1 extra
+    (R1W  : omap vala (reg r1) = Some w1)
+    (R2W  : omap vala (reg r2) = Some w2),
+    let lv := LVec STORE tpc ti [hseq r1; r2; w1] in forall
+    (NEXT : (do! st'  <- next_state_pc st lv (pc.+1);
+             let: State _ reg' pc' extra' := st' in
+             do! mem' <- repm mem w1 (fun v => w2@(taga v));
+             Some (State mem' reg' pc' extra')) = Some st'),  step st st'
+| step_jump : forall mem reg pc tpc i ti r w extra
     (ST   : st = State mem reg pc@tpc extra)
     (PC   : mem pc = Some i@ti)
     (INST : decode_instr i = Some (Jump r))
-    (RW   : reg r = Some w@t1),
-    let mvec := IVec JUMP tpc ti [hseq t1] in forall
-    (NEXT : next_state_pc st mvec w = Some st'),    step st st'
-| step_bnz : forall mem reg pc i r n w tpc ti t1 extra
+    (RW   : omap vala (reg r) = Some w),
+    let lv := LVec JUMP tpc ti [hseq r] in forall
+    (NEXT : next_state_pc st lv w = Some st'),    step st st'
+| step_bnz : forall mem reg pc tpc i ti r n w extra
     (ST   : st = State mem reg pc@tpc extra)
     (PC   : mem pc = Some i@ti)
     (INST : decode_instr i = Some (Bnz r n))
-    (RW   : reg r = Some w@t1),
-     let mvec := IVec BNZ tpc ti [hseq t1] in
-     let pc' := pc + (if w == 0%w
-                      then 1%w else swcast n) in forall
-    (NEXT : next_state_pc st mvec pc' = Some st'),     step st st'
-| step_jal : forall mem reg pc i r w tpc ti t1 old told extra
+    (RW   : omap vala (reg r) = Some w),
+    let lv := LVec BNZ tpc ti [hseq r] in
+    let pc' := pc + if w == 0%w then 1%w else swcast n in forall
+    (NEXT : next_state_pc st lv pc' = Some st'),     step st st'
+| step_jal : forall mem reg pc tpc i ti r w extra
     (ST : st = State mem reg pc@tpc extra)
     (PC : mem pc = Some i@ti)
     (INST : decode_instr i = Some (Jal r))
-    (RW : reg r = Some w@t1)
-    (OLD : reg ra = Some old@told),
-     let mvec := IVec JAL tpc ti [hseq t1; told] in forall
-    (NEXT : next_state_reg_and_pc st mvec ra (pc.+1) w = Some st'), step st st'
+    (RW : omap vala (reg r) = Some w),
+    let lv := LVec JAL tpc ti [hseq r; ra] in forall
+    (NEXT : next_state_reg_and_pc st lv ra (pc.+1) w = Some st'), step st st'
 | step_syscall : forall mem reg pc sc tpc extra
     (ST : st = State mem reg pc@tpc extra)
     (PC : mem pc = None)
@@ -354,5 +369,5 @@ Arguments Symbolic.state mt {_}.
 Arguments Symbolic.State {_ _} _ _ _ _.
 Arguments Symbolic.syscall mt {_}.
 Arguments Symbolic.syscall_table mt {_}.
-Arguments Symbolic.IVec {tty} op _ _ _.
-Arguments Symbolic.OVec {tty op} _ _.
+Arguments Symbolic.MVec {tty} op _ _ _.
+Arguments Symbolic.LVec {mt sp} opL _ _ _.
